Some progress on examples/bytestring

examples/bytestring/prims.c
@@ -4,6 +4,60 @@
 #include <stdio.h>
 #include <string.h>
 
+/* BEGIN stuff copied from examples/uint63nat/prims.c that
+   should be moved into gc_stack.h or similar */
+#define BEGINFRAME(tinfo,n) {{{{{ \
+   value *_ALLOC, *_LIMIT; \
+   value __ROOT__[n];   \
+   struct stack_frame __FRAME__ = { NULL/*bogus*/, __ROOT__, tinfo->fp }; \
+   struct stack_frame *__PREV__; \
+   value __RTEMP__;
+
+#define ENDFRAME }}}}}
+
+#define LIVEPOINTERS0(tinfo, exp) (exp)
+
+#define LIVEPOINTERS1(tinfo, exp, a0) \
+   (tinfo->fp= &__FRAME__, __FRAME__.next=__ROOT__+1, \
+   __ROOT__[0]=(a0), __RTEMP__=(exp), (a0)=__ROOT__[0], \
+   __PREV__=__FRAME__.prev, tinfo->fp=__PREV__, __RTEMP__)
+
+#define LIVEPOINTERS2(tinfo, exp, a0, a1)	\
+  (tinfo->fp= &__FRAME__, __FRAME__.next=__ROOT__+2, \
+  __ROOT__[0]=(a0), __ROOT__[1]=(a1),		\
+  __RTEMP__=(exp),                              \
+  (a0)=__ROOT__[0], (a1)=__ROOT__[1],             \
+   __PREV__=__FRAME__.prev, tinfo->fp=__PREV__, __RTEMP__)
+
+#define LIVEPOINTERS3(tinfo, exp, a0, a1, a2)   \
+  (tinfo->fp= &__FRAME__, __FRAME__.next=__ROOT__+3,                       \
+  __ROOT__[0]=(a0), __ROOT__[1]=(a1), __ROOT__[2]=(a2),  \
+  __RTEMP__=(exp),                                       \
+  (a0)=__ROOT__[0], (a1)=__ROOT__[1], (a2)=__ROOT__[2],    \
+   __PREV__=__FRAME__.prev, tinfo->fp=__PREV__, __RTEMP__)
+
+#define LIVEPOINTERS4(tinfo, exp, a0, a1, a2, a3)	\
+  (tinfo->fp= &__FRAME__,  __FRAME__.next=__ROOT__+4,  \
+  __ROOT__[0]=(a0), __ROOT__[1]=(a1), __ROOT__[2]=(a2), __ROOT__[3]=(a3),  \
+  __RTEMP__=(exp),                                       \
+  (a0)=__ROOT__[0], (a1)=__ROOT__[1], (a2)=__ROOT__[2], (a3)=__ROOT__[3],    \
+   __PREV__=__FRAME__.prev, tinfo->fp=__PREV__, __RTEMP__)
+
+#define GC_SAVE1(n) \
+    if (!(_LIMIT=tinfo->limit, _ALLOC=tinfo->alloc, (n) <= _LIMIT-_ALLOC)) { \
+    tinfo->nalloc = (n);  \
+    LIVEPOINTERS1(tinfo,(garbage_collect(tinfo),(value)NULL),save0);	\
+  }
+
+#define GC_SAVE2(n) \
+    if (!(_LIMIT=tinfo->limit, _ALLOC=tinfo->alloc, (n) <= _LIMIT-_ALLOC)) { \
+    tinfo->nalloc = (n);  \
+    LIVEPOINTERS2(tinfo,(garbage_collect(tinfo),(value)NULL),save0,save1);  \
+  }
+
+/* END stuff copied from examples/uint63nat/prims.c */
+
+/*
 #define LIVEPOINTERS0(tinfo, exp) (exp)
 #define LIVEPOINTERS1(tinfo, exp, a) ({ \
   value __ROOT__[1] = { a }; \
@@ -41,15 +95,13 @@
   tinfo->fp = &__FRAME__; value __TEMP__ = exp; \
   a = __ROOT__[0]; b = __ROOT__[1]; c = __ROOT__[2]; d = __ROOT__[3]; \
   tinfo->fp = __FRAME__.prev; __TEMP__; })
+*/
 
-value bytestrlen(value s)
+size_t bytestrlen(value s)
 {
-  value *ptr = (value *) s;
-  value *headerptr = ptr - 1;
-  value header = *headerptr;
-  value words = header >> 10;
-  value bytes = words * sizeof(value);
-  value padding = (value) *((char *) s + (bytes - 1)) + 1;
+  size_t header = (size_t)((value*)s)[-1];
+  size_t bytes = (header >> 10) * sizeof(value);
+  size_t padding = *((char *) s + (bytes - 1)) + 1;
   return bytes - padding;
 }
 
@@ -150,63 +202,62 @@ value map(struct thread_info *tinfo, value f, value s)
 }
 */
 
-value append(struct thread_info *tinfo, value s1, value s2)
+value append(struct thread_info *tinfo, value save0, value save1)
+  /* args must be exactly these names for convenience of GC_SAVE2 */
 {
-  value len1 = bytestrlen(s1);
-  value len2 = bytestrlen(s2);
-  value sum = len1 + len2;
-  value mod = sum % sizeof(value);
-  value pad_length = sizeof(value) - (sum % sizeof(value));
-  value nalloc = (sum + pad_length) / sizeof(value) + 1;
-  if (!(nalloc <= tinfo->limit - tinfo->alloc)) {
-    tinfo->nalloc = nalloc;
-    LIVEPOINTERS2_(tinfo, garbage_collect(tinfo), s1, s2);
-  }
+  size_t i;
+  size_t len1 = bytestrlen(save0);
+  size_t len2 = bytestrlen(save1);
+  size_t sum = len1 + len2;
+  size_t mod = sum % sizeof(value);
+  size_t pad_length = sizeof(value) - (sum % sizeof(value));
+  size_t nalloc = (sum + pad_length) / sizeof(value) + 1;
+  BEGINFRAME(tinfo,2)
+  GC_SAVE2(nalloc) /* no semicolon */
 
-  value *argv = (value *) tinfo->alloc;
-  *((value *) argv + 0LLU) = ((nalloc - 1) << 10) + 252LLU; // string tag
+  value *argv = tinfo->alloc;
+  argv[0LLU] = (value*)(((nalloc - 1) << 10) + 252LLU); // string tag
   
   // take a pointer pointing to the beginning of destination string
   char *ptr = (char *) (argv + 1LLU);
-  char *t1 = (char *) s1;
-  char *t2 = (char *) s2;
+  char *t1 = (char *) save0;
+  char *t2 = (char *) save1;
 
   // copy the OCaml-string pointed by t1 and t2
   // into the array pointed by ptr
   // skip the padding in each one, we'll make our own padding later
-  for (value i = 0; i < len1; i++) { *ptr = *t1; ptr++; t1++; }
-  for (value i = 0; i < len2; i++) { *ptr = *t2; ptr++; t2++; }
+  for (i = 0; i < len1; i++) ptr[i]=t1[i];
+  for (i = 0; i < len2; i++) ptr[len1+i]=t2[i];
 
   // make the padding
-  char i = 0;
-  while (i < pad_length - 1) { *ptr = 0; ptr++; i++; }
-  *ptr = i; // last char in the padding is # of 0s coming before the last char
-
+  for (i=0; i < pad_length - 1; i++) ptr[len1+len2+i]=0;
+  ptr[len1+len2+(pad_length-1)] = pad_length-1;
+       // last char in the padding is # of 0s coming before the last char
   tinfo->alloc += nalloc;
   return (value) (argv + 1LLU);
+  ENDFRAME
 }
 
-value pack(struct thread_info *tinfo, value s)
+value pack(struct thread_info *tinfo, value save0)
+  /* args must be exactly these names for convenience of GC_SAVE1 */
 {
-  value temp = s;
-  value len = 0;
+  BEGINFRAME(tinfo,1)
+  value temp = save0;
+  size_t i, len = 0;
   while(get_Coq_Strings_String_string_tag(temp) == 1) {
     len++;
     temp = *((value *) temp + 1ULL);
   } 
-  value mod = len % sizeof(value);
-  value pad_length = sizeof(value) - (len % sizeof(value));
-  value nalloc = (len + pad_length) / sizeof(value) + 1;
-  if (!(nalloc <= tinfo->limit - tinfo->alloc)) {
-    tinfo->nalloc = nalloc;
-    LIVEPOINTERS1_(tinfo, garbage_collect(tinfo), s);
-  }
+  size_t mod = len % sizeof(value);
+  size_t pad_length = sizeof(value) - (len % sizeof(value));
+  size_t nalloc = (len + pad_length) / sizeof(value) + 1ULL;
+  GC_SAVE1(nalloc) /* no semicolon */
 
-  value *argv = (value *) tinfo->alloc;
-  *((value *) argv + 0LLU) = ((nalloc - 1) << 10) + 252LLU; // string tag
+  value *argv = tinfo->alloc;
+  argv[0LLU] = (value)(((nalloc - 1) << 10) + 252LLU); // string tag
 
   char *ptr = (char *) (argv + 1LLU);
-  temp = s;
+  temp = save0;
   while(get_Coq_Strings_String_string_tag(temp) == 1) {
     *ptr = ascii_to_char(temp);
     ptr++;
@@ -214,36 +265,42 @@ value pack(struct thread_info *tinfo, value s)
   } 
 
   // make the padding
-  char i = 0;
-  while (i < pad_length - 1) { *ptr = 0; ptr++; i++; }
-  *ptr = i; // last char in the padding is # of 0s coming before the last char
+  
+  for (i=0; i<pad_length-1; i++) ptr[i]=0;
+  ptr[i]=i;
 
   tinfo->alloc += nalloc;
   return (value) (argv + 1LLU);
+  ENDFRAME
 }
 
 
-value unpack(struct thread_info *tinfo, value bs)
-{
-  // 3 for the String constructor, 9 for the ASCII constructor.
-  value nalloc = bytestrlen(bs) * (3 + 9);
-  if (!(nalloc <= tinfo->limit - tinfo->alloc)) {
-    tinfo->nalloc = nalloc;
-    LIVEPOINTERS1_(tinfo, garbage_collect(tinfo), bs);
-  }
 
-  char *s = (char *) bs;
-  value temp = make_Coq_Strings_String_string_EmptyString();
-  for (unsigned int i = bytestrlen(bs); 0 < i; i--) {
-    value c = char_to_value(tinfo, s[i-1]);
-    temp = alloc_make_Coq_Strings_String_string_String(tinfo, c, temp);
+value unpack(struct thread_info *tinfo, value save0)
+  /* args and save1 must be exactly these names for convenience of GC_SAVE2 */
+{
+  char c; value v;
+  size_t len = bytestrlen(save0);
+  value save1 = make_Coq_Strings_String_string_EmptyString();
+  BEGINFRAME(tinfo,2)
+  while (len--) {
+    GC_SAVE2(12)   // 3 for the String constructor, 9 for the ASCII constructor.
+    c = ((char*)save1)[len];
+    v = char_to_value(tinfo, c);
+    save1 = alloc_make_Coq_Strings_String_string_String(tinfo, v, save1);
   }
-  return temp;
+  return save1;
+  ENDFRAME
 }
 
 // from https://codereview.stackexchange.com/a/207541/68819
 // allocates enough memory for a string (which has to be freed later)
 // returns its length by assigning it to the pointer in the argument
+
+extern void * malloc(size_t size);
+extern void *realloc(void *ptr, size_t size);
+extern void free(void *ptr);
+
 char *scan(FILE *stream, size_t *length)
 {
   size_t capacity = 16;
@@ -279,21 +336,19 @@ char *scan(FILE *stream, size_t *length)
   return buffer;
 }
 
-value scan_bytestring(struct thread_info *tinfo, value instream)
+value scan_bytestring(struct thread_info *tinfo, value save0)
 {
+  BEGINFRAME(tinfo,1)
   size_t len;
-  char *s = scan((FILE *) instream, &len);
+  char *s = scan((FILE *) save0, &len);
 
-  value mod = len % sizeof(value);
-  value pad_length = sizeof(value) - (len % sizeof(value));
-  value nalloc = (len + pad_length) / sizeof(value) + 1;
-  if (!(nalloc <= tinfo->limit - tinfo->alloc)) {
-    tinfo->nalloc = nalloc;
-    LIVEPOINTERS1_(tinfo, garbage_collect(tinfo), instream);
-  }
+  size_t mod = len % sizeof(value);
+  size_t pad_length = sizeof(value) - (len % sizeof(value));
+  size_t nalloc = (len + pad_length) / sizeof(value) + 1;
+  GC_SAVE1(nalloc)  /* no semicolon */
 
-  value *argv = (value *) tinfo->alloc;
-  *((value *) argv + 0LLU) = ((nalloc - 1) << 10) + 252LLU; // string tag
+  value *argv = tinfo->alloc;
+  *((value *) argv + 0LLU) = (value)(((nalloc - 1) << 10) + 252LLU); // string tag
 
   char *ptr = (char *) (argv + 1LLU);
   char *t = (char *) s;
@@ -306,6 +361,7 @@ value scan_bytestring(struct thread_info *tinfo, value instream)
 
   tinfo->alloc += nalloc;
   return (value) (argv + 1LLU);
+  ENDFRAME
 }
 
 /////////////////////////////////////////////////////////////////
@@ -314,20 +370,25 @@ typedef enum { PURE, BIND, PRINT, SCAN } M;
 value runM(struct thread_info * tinfo, value a, value instream, value outstream, value action)
 {
   value temp, arg0, arg1;
+  BEGINFRAME(tinfo,4)
   switch (get_prog_C_MI_tag(action)) {
     case PURE:
       return get_args(action)[1];
     case BIND:
-      arg0 = get_args(action)[2];
-      arg1 = get_args(action)[3];
-      temp = LIVEPOINTERS4(tinfo, runM(tinfo, a, instream, outstream, arg0), arg0, arg1, instream, outstream);
-      temp = LIVEPOINTERS4(tinfo, call(tinfo, arg1, temp), arg1, instream, outstream, temp);
+      temp = LIVEPOINTERS4(tinfo,
+			   (arg0 = get_args(action)[2],
+                            runM(tinfo, a, instream, outstream, arg0)),
+			   action,instream,outstream,a);
+      temp = LIVEPOINTERS3(tinfo,
+			   (arg1 = get_args(action)[3],
+			    call(tinfo,arg1,temp)),
+			   instream, outstream,a);
       return runM(tinfo, a, instream, outstream, temp);
     case PRINT:
       {
         value s = *((value *) action);
-        value len = bytestrlen(s);
-        for (value i = 0; i < len; i ++) {
+        size_t len = bytestrlen(s);
+        for (size_t i = 0; i < len; i ++) {
           fprintf((FILE *) outstream, "%c", ((char *) s)[i]);
         }
         fprintf((FILE *) outstream, "\n");
@@ -338,12 +399,13 @@ value runM(struct thread_info * tinfo, value a, value instream, value outstream,
     default:
       return 0;
   }
+  ENDFRAME
 }
 
 value get_stdin(struct thread_info * tinfo, value _tt) {
-  return stdin;
+  return (value)stdin;
 }
 
 value get_stdout(struct thread_info * tinfo, value _tt) {
-  return stdout;
+  return (value)stdout;
 }
